cedar-lean/Cedar/Thm/SymCC/Opt/Extractor.lean
@@ -26,111 +26,109 @@ namespace Cedar.Thm
 
 open Cedar.Spec Cedar.SymCC
 
-theorem cp_extractOpt?_eqv_extract? {cps : List CompiledPolicy} {I : Interpretation} {εnv : SymEnv} :
-  cps ≠ [] →
-  (∀ cp ∈ cps, cp.εnv = εnv) →
-  -- the `CompiledPolicy`s at least have to be constructed with `CompiledPolicy.compile`, even though we don't care about the original uncompiled policies
-  (∀ cp ∈ cps, ∃ p Γ, CompiledPolicy.compile p Γ = .ok cp) →
-  CompiledPolicy.extractOpt? cps I = SymEnv.extract? (cps.map (Policy.toExpr ∘ CompiledPolicy.policy)) I εnv
+theorem extractOpt?_eqv_extract? {cpₛs : List CompiledPolicyₛ} {I : Interpretation} {εnv : SymEnv} :
+  cpₛs ≠ [] →
+  (∀ cpₛ ∈ cpₛs, cpₛ.εnv = εnv) →
+  -- the `CompiledPolicyₛ` at least have to be constructed with `CompiledPolicy.compile` or `CompiledPolicies.compile`, even though we don't care about the original uncompiled policies
+  (∀ cpₛ ∈ cpₛs, match cpₛ with
+    | .policy cp => ∃ p Γ, CompiledPolicy.compile p Γ = .ok cp
+    | .policies cps => ∃ ps Γ, CompiledPolicies.compile ps Γ = .ok cps
+  ) →
+  extractOpt? cpₛs I = SymEnv.extract? ((cpₛs.flatMap CompiledPolicyₛ.allPolicies).map Policy.toExpr) I εnv
 := by
-  simp [CompiledPolicy.extractOpt?, SymEnv.extract?]
+  simp [extractOpt?, SymEnv.extract?]
   intro hnil hεnv hcompile
-  split
-  · simp at hnil
-  · rename_i term εnv' policy footprint acyclicity cps
-    simp only [List.mem_cons, forall_eq_or_imp] at hεnv
-    replace ⟨hεnv', hεnv⟩ := hεnv ; subst εnv'
-    simp_all only [reduceCtorEq, not_false_eq_true, List.map_cons, Function.comp_apply, footprints]
-    congr 3
+  simp only [CompiledPolicyₛ.εnv] at hεnv
+  split <;> simp_all only [reduceCtorEq, not_true_eq_false, not_false_eq_true, List.mem_cons,
+    forall_eq_or_imp, List.flatMap_cons, List.map_append, footprints]
+  rename_i cpₛ cpₛs
+  replace ⟨hεnv', hεnv⟩ := hεnv
+  congr 3
+  cases cpₛ <;> simp_all only [CompiledPolicyₛ.allPolicies, List.map_cons, List.map_nil,
+    List.cons_append, List.nil_append]
+  all_goals {
+    subst εnv
+    first | rename CompiledPolicy => cp | rename CompiledPolicies => cps
+    replace ⟨⟨p, Γ, hcompile⟩, hcompile'⟩ := hcompile ; try rename Policies => ps
     rw [List.mapUnion_cons]
-    · rw [List.mapUnion_cons]
-      · congr 1
-        · replace ⟨p, Γ, hcompile⟩ := hcompile { term, εnv, policy, footprint, acyclicity } (by simp)
-          apply cp_compile_produces_the_right_footprint hcompile
-        · rw [List.mapUnion_map]
-          apply List.mapUnion_congr
-          intro cp hcp
-          replace ⟨p, Γ, hcompile⟩ := hcompile cp (by simp [hcp])
-          simp [cp_compile_produces_the_right_footprint hcompile, hεnv cp hcp]
-      · intro x hx
-        cases hx <;> apply footprint_wf
-    · intro cp hcp
-      cases hcp
-      · replace ⟨p, Γ, hcompile⟩ := hcompile { term, εnv, policy, footprint, acyclicity } (by simp)
-        have := cp_compile_produces_the_right_footprint hcompile ; simp at this ; subst footprint
-        simp [footprint_wf]
-      · rename_i hcp
-        replace ⟨p, Γ, hcompile⟩ := hcompile cp (by right ; simp [hcp])
-        simp [cp_compile_produces_the_right_footprint hcompile]
-        apply footprint_wf
-
-theorem cps_extractOpt?_eqv_extract? {cpss : List CompiledPolicies} {I : Interpretation} {εnv : SymEnv} :
-  cpss ≠ [] →
-  (∀ cps ∈ cpss, cps.εnv = εnv) →
-  -- the `CompiledPolicies` at least have to be constructed with `CompiledPolicies.compile`, even though we don't care about the original uncompiled policies
-  (∀ cps ∈ cpss, ∃ ps Γ, CompiledPolicies.compile ps Γ = .ok cps) →
-  CompiledPolicies.extractOpt? cpss I = SymEnv.extract? ((cpss.flatMap CompiledPolicies.policies).map Policy.toExpr) I εnv
-:= by
-  simp [CompiledPolicies.extractOpt?, SymEnv.extract?]
-  intro hnil hεnv hcompile
-  split
-  · simp at hnil
-  · rename_i term εnv' policies footprint acyclicity cpss
-    simp only [List.mem_cons, forall_eq_or_imp] at hεnv
-    replace ⟨hεnv', hεnv⟩ := hεnv ; subst εnv'
-    simp_all only [reduceCtorEq, not_false_eq_true, List.mem_cons, forall_eq_or_imp, List.map_cons,
-      Function.comp_apply, List.flatten_cons, List.flatMap_cons, List.map_append, footprints]
-    congr 3
-    · grind
-    · replace ⟨⟨ps, Γ, hcompile⟩, hcompile'⟩ := hcompile
-      rw [List.mapUnion_cons]
-      · rw [List.mapUnion_append (by simp [footprint_wf])]
-        rw [List.mapUnion_map, List.mapUnion_map]
-        simp only [Union.union, HAppend.hAppend]
-        congr 1
-        · have := cps_compile_produces_the_right_footprint hcompile ; simp at this ; subst footprint
-          simp only [footprints]
-          apply List.mapUnion_map
-        · rw [← Data.Set.eq_means_eqv List.mapUnion_wf List.mapUnion_wf]
-          simp [List.Equiv, List.subset_def]
-          constructor
-          · intro t
-            simp only [Data.Set.in_list_iff_in_set]
-            simp only [List.mem_mapUnion_iff_mem_exists t, List.mem_flatMap,
-              Function.comp_apply, forall_exists_index, and_imp]
-            intro cps hcps ht
-            replace ⟨ps', Γ', hcompile'⟩ := hcompile' cps hcps
+    · simp only [CompiledPolicyₛ.footprint]
+      first
+      | rw [List.mapUnion_cons (by simp [footprint_wf])]
+      | rw [List.mapUnion_append (by simp [footprint_wf])]
+      congr 1
+      · first
+        | apply cp_compile_produces_the_right_footprint hcompile
+        | apply cps_compile_produces_the_right_footprint hcompile
+      · rw [List.mapUnion_map]
+        rw [← Data.Set.eq_means_eqv List.mapUnion_wf List.mapUnion_wf]
+        simp only [List.Equiv, List.subset_def, Data.Set.in_list_iff_in_set,
+          List.mem_mapUnion_iff_mem_exists, List.mem_flatMap, Function.comp_apply,
+          forall_exists_index, and_imp]
+        constructor
+        · intro t cpₛ hcpₛ ht
+          specialize hcompile' cpₛ hcpₛ
+          split at hcompile'
+          · rename_i cpₛ cp
+            replace ⟨p', Γ', hcompile'⟩ := hcompile'
+            have hfoot := cp_compile_produces_the_right_footprint hcompile'
+            simp [CompiledPolicyₛ.footprint, hfoot] at ht
+            exists cp.policy
+            specialize hεnv (.policy cp) hcpₛ ; simp only at hεnv ; rw [← hεnv]
+            simp only [ht, and_true]
+            exists .policy cp
+            simp [hcpₛ, CompiledPolicyₛ.allPolicies]
+          · rename_i cpₛ cps
+            replace ⟨ps', Γ', hcompile'⟩ := hcompile'
             have hfoot := cps_compile_produces_the_right_footprint hcompile'
-            simp only [footprints] at hfoot
-            rw [List.mapUnion_map, ← Data.Set.eq_means_eqv] at hfoot
-            · simp [List.Equiv, List.subset_def, Data.Set.in_list_iff_in_set] at hfoot
+            simp only [footprints, List.mapUnion_map] at hfoot
+            rw [← Data.Set.eq_means_eqv] at hfoot
+            · simp only [List.Equiv, List.subset_def, Data.Set.in_list_iff_in_set] at hfoot
               replace ⟨hfoot, hfoot'⟩ := hfoot
               specialize hfoot ht
               rw [List.mem_mapUnion_iff_mem_exists] at hfoot
               replace ⟨p, hp, hfoot⟩ := hfoot
               exists p
-              rw [hεnv cps hcps] at *
-              grind
+              specialize hεnv (.policies cps) hcpₛ ; simp only at hεnv ; rw [← hεnv]
+              simp only [Function.comp_apply] at hfoot
+              simp only [hfoot, and_true]
+              exists .policies cps
             · simp [hfoot, List.mapUnion_wf]
             · simp [List.mapUnion_wf]
-          · intro t
-            simp only [Data.Set.in_list_iff_in_set]
-            simp only [List.mem_mapUnion_iff_mem_exists t, List.mem_flatMap,
-              Function.comp_apply, forall_exists_index, and_imp]
-            intro p cps hcps hp ht
-            exists cps
-            replace ⟨ps', Γ', hcompile'⟩ := hcompile' cps hcps
+        · intro t p cpₛ hcpₛ hp ht
+          exists cpₛ
+          specialize hcompile' cpₛ hcpₛ
+          split at hcompile'
+          · rename_i cpₛ cp
+            simp only [CompiledPolicyₛ.allPolicies, List.mem_cons, List.not_mem_nil,
+              or_false] at hp ; subst p
+            replace ⟨p', Γ', hcompile'⟩ := hcompile'
+            have hfoot := cp_compile_produces_the_right_footprint hcompile'
+            simp only [hcpₛ, CompiledPolicyₛ.footprint, hfoot, true_and]
+            specialize hεnv (.policy cp) hcpₛ ; simp only at hεnv ; rw [← hεnv] at ht
+            exact ht
+          · rename_i cpₛ cps
+            simp only [CompiledPolicyₛ.allPolicies] at hp
+            replace ⟨ps', Γ', hcompile'⟩ := hcompile'
             have hfoot := cps_compile_produces_the_right_footprint hcompile'
-            simp only [hcps, hfoot, footprints, true_and]
-            rw [hεnv cps hcps] at *
+            simp only [hcpₛ, CompiledPolicyₛ.footprint, hfoot, footprints, true_and]
+            specialize hεnv (.policies cps) hcpₛ ; simp only at hεnv ; rw [← hεnv] at ht
             apply List.mem_mem_implies_mem_mapUnion (s := p.toExpr) ht
             simp only [List.mem_map]
             exists p
-      · intro cps hcps
-        cases hcps
-        · have := cps_compile_produces_the_right_footprint hcompile ; simp at this ; subst footprint
-          simp [footprints_wf]
-        · rename_i hcps
-          have ⟨ps, Γ, hcompile'⟩ := hcompile' cps hcps
-          have := cps_compile_produces_the_right_footprint hcompile'
-          simp [this, footprints_wf]
+    · intro cpₛ hcpₛ
+      cases hcpₛ
+      · first
+        | have := cp_compile_produces_the_right_footprint hcompile
+        | have := cps_compile_produces_the_right_footprint hcompile
+        simp only at this
+        simp [CompiledPolicyₛ.footprint, this, footprint_wf, footprints_wf]
+      · rename_i hcpₛ
+        specialize hcompile' cpₛ hcpₛ
+        split at hcompile'
+        · rename_i cpₛ cp
+          replace ⟨p, Γ, hcompile'⟩ := hcompile'
+          simp [CompiledPolicyₛ.footprint, cp_compile_produces_the_right_footprint hcompile', footprint_wf]
+        · rename_i cpₛ cps
+          replace ⟨ps, Γ, hcompile'⟩ := hcompile'
+          simp [CompiledPolicyₛ.footprint, cps_compile_produces_the_right_footprint hcompile', footprints_wf]
+  }
